Church.v
@@ -162,4 +162,53 @@ Proof.
 Qed.
 
 
+Lemma WCT_WRTw :
+  WCT_Q -> WRT_weak.
+Proof.
+  intros wct p [f Hf]%enumerable_nat.
+  apply (DN_chaining (wct f)), DN.
+  intros [ϕ [b2 [[s1] H]]].
+  pose (Φ := ϕ[up (σ $1)..] ).
+  exists Φ; split. 2: split.
+  - unfold Φ. eapply subst_bound; eauto.
+    intros [|[|[]]]; cbn; repeat solve_bounds.
+  - constructor. now apply subst_delta0. 
+  - intros x. rewrite Hf. split.
+    + intros [n Hn]. symmetry in Hn.
+      apply Σ1_ternary_complete.
+      { unfold Φ. eapply subst_bound; eauto.
+      intros [|[|[]]]; cbn; repeat solve_bounds. }
+      { now apply subst_delta0. } 
+      exists n. specialize (H n).
+      apply soundness in H.
+      unshelve refine (let H := (H nat interp_nat (fun _ => 0)) _ in _ ).
+      {apply Q_std_axioms. }
+      cbn in H. specialize (H (S x)) as [_ H2].
+      rewrite eval_num, inu_nat_id in *.
+      apply H2 in Hn. destruct Hn as [d Hd].
+      exists d.
+      unfold Φ. rewrite !sat_comp in *.
+      eapply bound_ext with (N:=3).
+      apply b2. 2: apply Hd.
+      intros [|[|[]]]; cbn; rewrite ?num_subst, ?eval_num, ?inu_nat_id in *.
+      all: try lia; reflexivity.
+    + intros HQ%soundness. specialize (HQ nat interp_nat (fun _ => 0)).
+      destruct HQ as [n [d Hnd]].
+      {apply Q_std_axioms. }
+      exists n. specialize (H n).
+      apply soundness in H.
+      unshelve refine (let H := (H nat interp_nat (fun _ => 0)) _ in _ ).
+      apply Q_std_axioms.
+      cbn in H. specialize (H (S x)) as [H1 _].
+      rewrite eval_num, inu_nat_id in *.
+      symmetry. apply H1. exists d.
+      rewrite !sat_comp in Hnd. 
+      unfold Φ in Hnd. rewrite sat_comp in *.
+      eapply bound_ext.
+      apply b2. 2: apply Hnd.
+      intros [|[|[]]]; cbn; rewrite ?num_subst, ?eval_num, ?inu_nat_id in *.
+      all: try lia; reflexivity.
+Qed.
+
+
 End ChurchThesis.
